src/dvspec/dafny/att_spec_proofs/assump.dfy
@@ -15,50 +15,73 @@ module AttAssumptions
     import opened DV
     import opened AttInvariants
     
+    // Assumption 4a
+    // Let a be a new attestation duty served to an honest node n. Then
+    // either a is the first served duty of n or 
+    // a’s slot is greater than the slot of the latest served duty served by n.
     lemma {:axiom}  monotonic_seq_of_rcvd_att_duties<D(!new, 0)>(
+        dvn: DVState,
+        pubkey: BLSPubkey,        
+        new_att_duty: AttestationDuty)       
+    requires && is_honest_node(dvn, pubkey) 
+             && var s := dvn.honest_nodes_states[pubkey];
+             && f_serve_attestation_duty.requires(s, new_att_duty)
+    ensures && var s := dvn.honest_nodes_states[pubkey];
+            && ( || !s.latest_attestation_duty.isPresent()
+                 || ( && s.latest_attestation_duty.isPresent()
+                      && s.latest_attestation_duty.safe_get().slot < new_att_duty.slot 
+                    )
+               )
+
+    // Assumption 4b
+    // Let a be a new attestation duty served to an honest node n. 
+    // For every honest node n1, for every duty d that n1 received, if d’s
+    // slot is less than a’s slot, then n received d.
+    lemma {:axiom}  rcvd_att_duties_as_prefixes<D(!new, 0)>(
         dvn: DVState,
         pubkey: BLSPubkey,
         s: DVCNodeState,
         new_att_duty: AttestationDuty)       
-    requires is_honest_node(dvn, pubkey) && s == dvn.honest_nodes_states[pubkey]
-    requires f_serve_attestation_duty.requires(s, new_att_duty)
-    ensures || !s.latest_attestation_duty.isPresent()
-            || ( && s.latest_attestation_duty.isPresent()
-                 && s.latest_attestation_duty.safe_get().slot < new_att_duty.slot 
-               )
-    
+    requires && is_honest_node(dvn, pubkey) 
+             && var s := dvn.honest_nodes_states[pubkey];
+             && f_serve_attestation_duty.requires(s, new_att_duty)
+    ensures && var s := dvn.honest_nodes_states[pubkey];
+            && forall p1: BLSPubkey, duty: AttestationDuty :: 
+                    && is_honest_node(dvn, p1)
+                    && var s1 := dvn.honest_nodes_states[p1];
+                    && duty in s1.all_rcvd_duties
+                    && duty.slot < new_att_duty.slot
+                        ==> duty in s.all_rcvd_duties
+
+    // Assumption 4c
+    // Let a be a new attestation duty served to an honest node n. Then
+    //    - Either for every honest node n1, for every duty d that n1 received,
+    //      d’s slot is less than a’s slot.
+    //    - Or there exits an honest node n1 such that n1 received a.
     lemma {:axiom}  rcvd_att_duties_is_prefix_of_global_att_duties<D(!new, 0)>(
         dvn: DVState,
         pubkey: BLSPubkey,
         s: DVCNodeState,
         new_att_duty: AttestationDuty)       
-    requires is_honest_node(dvn, pubkey) && s == dvn.honest_nodes_states[pubkey]
-    requires f_serve_attestation_duty.requires(s, new_att_duty)
-    ensures || ( exists p1: BLSPubkey :: 
-                    && is_honest_node(dvn, p1)
-                    && var s1 := dvn.honest_nodes_states[p1];
-                    && s1.latest_attestation_duty.isPresent()
-                    && s1.latest_attestation_duty.safe_get() == new_att_duty
+    requires && is_honest_node(dvn, pubkey) 
+             && var s := dvn.honest_nodes_states[pubkey];
+             && f_serve_attestation_duty.requires(s, new_att_duty)
+    ensures && var s := dvn.honest_nodes_states[pubkey];
+            && ( || ( forall p1: BLSPubkey, duty: AttestationDuty :: 
+                          && is_honest_node(dvn, p1)
+                          && var s1 := dvn.honest_nodes_states[p1];                    
+                          && duty in s1.all_rcvd_duties
+                              ==> duty.slot < new_att_duty.slot                                                   
+                    )
+                  || ( exists p1: BLSPubkey :: 
+                          && is_honest_node(dvn, p1)
+                          && var s1 := dvn.honest_nodes_states[p1];
+                          && s1.latest_attestation_duty.isPresent()
+                          && new_att_duty in s1.all_rcvd_duties
+                     )
                )
-            || ( forall p1: BLSPubkey :: 
-                    && is_honest_node(dvn, p1)
-                    && var s1 := dvn.honest_nodes_states[p1];                    
-                    && ( || !s1.latest_attestation_duty.isPresent()
-                         || ( && s1.latest_attestation_duty.isPresent()
-                              && s1.latest_attestation_duty.safe_get().slot < new_att_duty.slot
-                            )
-                       )
-               )
-    ensures ! ( exists duty: AttestationDuty ::
-                    && ! ( duty in s.all_rcvd_duties ) 
-                    && duty.slot < new_att_duty.slot
-                    && exists p1: BLSPubkey :: 
-                            ( && is_honest_node(dvn, p1)
-                              && var s1 := dvn.honest_nodes_states[p1];                     
-                              && duty in s1.all_rcvd_duties
-                            )
-              )
-    
+            
+  // Assumption 5
   lemma {:axiom} constructable_signed_attestation_signature(
     dvn: DVState,
     att_shares: set<AttestationShare>) 
@@ -71,6 +94,7 @@ module AttAssumptions
                             && s2 in S
                                 ==> att_shares_from_same_att_data(s1, s2) )
 
+  // Assumption 6
   lemma {:axiom} agreement_on_constructed_signed_attestation_signature(
     dvn: DVState,
     att_shares1: set<AttestationShare>, 
@@ -87,7 +111,12 @@ module AttAssumptions
                     && ( forall s1, s2: AttestationShare ::
                             && s1 in S
                             && s2 in S
-                                ==> att_shares_from_same_att_data(s1, s2) )                                
+                                ==> att_shares_from_same_att_data(s1, s2) ) 
+
+  lemma {:axiom} init_satisfies_ByzThresholdAssumption(dvn: DVState)       
+  requires exists initial_attestation_slashing_db: set<SlashingDBAttestation> :: 
+                DV.Init(dvn, initial_attestation_slashing_db)        
+  ensures ByzThresholdAssumption(dvn.all_nodes, dvn.honest_nodes_states.Keys, dvn.adversary.nodes)                                                            
 }
 
 
